Progress in proving fuel-free erasure function

extraction/theories/Extract.v
@@ -18,13 +18,15 @@ Definition is_prop_sort s :=
   | None => false
   end.
 
-Parameter is_type_or_proof : forall (Sigma : global_context) (Gamma : context) (t : PCUICAst.term), bool.
+Parameter is_type_or_proof : forall (Σ : global_context), wf Σ -> forall (Γ : context), wf_local Σ Γ -> forall (t : PCUICAst.term), typing_result bool.
 From MetaCoq.PCUIC Require Import PCUICTyping.
 
 Definition Is_Type_or_Proof Σ Γ t := ∑ T, Σ ;;; Γ |- t : T × (isArity T + (∑ u, (Σ ;;; Γ |- T : tSort u) * is_prop_sort u))%type.
 
-Axiom is_type_or_proof_spec : forall (Sigma : global_context) (Gamma : context) (t : PCUICAst.term) T,
-    Sigma ;;; Gamma |- t : T -> (is_type_or_proof Sigma Gamma t = true) <~> Is_Type_or_Proof Sigma Gamma t.
+Axiom is_type_or_proof_spec : forall (Sigma : global_context) wfΣ (Gamma : context) wfΓ (t : PCUICAst.term) T b,
+    Sigma ;;; Gamma |- t : T ->
+    is_type_or_proof Sigma wfΣ Gamma wfΓ t = Checked b ->
+    (b = true) <~> Is_Type_or_Proof Sigma Gamma t.
 
 (* Section IsType. *)
 (*   Context {F : Fuel}. *)
@@ -83,14 +85,14 @@ Definition Informative (Σ : global_context) (ind : inductive) :=
 Module E := EAst.
 Local Notation Ret t := t.
 
-Section Erase.
-  (* Context `{F : Fuel}. *)
 
-  Definition is_box c :=
-    match c with
-    | E.tBox => true
-    | _ => false
-    end.
+(* Section Erase. *)
+
+(*   Definition is_box c := *)
+(*     match c with *)
+(*     | E.tBox => true *)
+(*     | _ => false *)
+(*     end. *)
 
   Fixpoint mkAppBox c n :=
     match n with
@@ -98,85 +100,159 @@ Section Erase.
     | S n => mkAppBox (E.tApp c E.tBox) n
     end.
 
-  Definition on_snd_map {A B C} (f : B -> C) (p : A * B) :=
-    (fst p, f (snd p)).
+(*   Definition on_snd_map {A B C} (f : B -> C) (p : A * B) := *)
+(*     (fst p, f (snd p)). *)
 
-  Section EraseMfix.
-    Context (extract : forall (Γ : context) (t : term), E.term).
+(*   Section EraseMfix. *)
+(*     Context (extract : forall Σ (wfΣ : wf Σ ) (Γ : context) (wfΓ : wf_local Σ Γ) (t : term), typing_result E.term). *)
 
-    Definition extract_mfix Γ (defs : mfixpoint term) : (EAst.mfixpoint E.term) :=
-      let Γ' := (PCUICLiftSubst.fix_context defs ++ Γ)%list in
-      map (fun d => let dbody' := extract Γ' d.(dbody) in
-                          Ret ({| E.dname := d.(dname); E.rarg := d.(rarg);
-                                  E.dbody := dbody' |})) defs.
-  End EraseMfix.
+(*     Program Definition extract_mfix Σ wfΣ Γ (wfΓ : wf_local Σ Γ) (defs : mfixpoint term) : typing_result (EAst.mfixpoint E.term) := *)
+(*       let Γ' := (fix_decls defs ++ Γ)%list in *)
+(*       monad_map (fun d => dbody' <- extract Σ wfΣ Γ' _ d.(dbody);; *)
+(*                           ret ({| E.dname := d.(dname); E.rarg := d.(rarg); *)
+(*                                   E.dbody := dbody' |})) defs. *)
+(*     Next Obligation. *)
+(*     Admitted. *)
+          
+(*   End EraseMfix. *)
   
-  Fixpoint extract (Σ : global_context) (Γ : context) (t : term) : E.term :=
-    if is_type_or_proof Σ Γ t then E.tBox else
-    match t with
-    | tRel i => Ret (E.tRel i)
-    | tVar n => Ret (E.tVar n)
-    | tEvar m l =>
-      Ret (E.tEvar m (map (extract Σ Γ) l))
-    | tSort u => Ret E.tBox
-    | tConst kn u => Ret (E.tConst kn)
-    | tInd kn u => Ret E.tBox
-    | tConstruct kn k u => Ret (E.tConstruct kn k)
-    | tProd na b t => Ret E.tBox
-    | tLambda na b t =>
-      let t' := extract Σ (vass na b :: Γ) t in
-      Ret (E.tLambda na t')
-    | tLetIn na b t0 t1 =>
-      let b' := extract Σ Γ b in
-      let t1' := extract Σ (vdef na b t0 :: Γ) t1 in
-      Ret (E.tLetIn na b' t1')
-    | tApp f u =>
-      let f' := extract Σ Γ f in
-      let l' := extract Σ Γ u in
-      Ret (E.tApp f' l') (* if is_dummy f' then Ret dummy else *)
-    | tCase ip p c brs =>
-      let c' := extract Σ Γ c in
-      (* if is_box c' then *)
-      (*   match brs with *)
-      (*   | (n, x) :: _ => *)
-      (*     let x' := extract Σ Γ x in *)
-      (*     Ret (mkAppBox x' n) (* Singleton elimination *) *)
-      (*   | nil => *)
-      (*     Ret (E.tCase ip c' nil) (* Falsity elimination *) *)
-      (*   end *)
-      (* else *)
-        let brs' := map (B := nat * E.term) (fun x => let x' := extract Σ Γ (snd x) in Ret (fst x, x')) brs in
-        Ret (E.tCase ip c' brs')
-    | tProj p c =>
-      let c' := extract Σ Γ c in
-      Ret (E.tProj p c')
-    | tFix mfix n =>
-      let mfix' := extract_mfix (extract Σ) Γ mfix in
-      Ret (E.tFix mfix' n)
-    | tCoFix mfix n =>
-      let mfix' := extract_mfix (extract Σ) Γ mfix in
-      Ret (E.tCoFix mfix' n)
-    end.
+(*   Program Fixpoint extract (Σ : global_context) {wfΣ : wf Σ} (Γ : context) {wfΓ : wf_local Σ Γ} (t : term) {struct t} : typing_result E.term := *)
+(*     b <- is_type_or_proof Σ wfΣ Γ wfΓ t ;; *)
+(*     if (b : bool) then ret E.tBox else *)
+(*     match t with *)
+(*     | tRel i => ret (E.tRel i) *)
+(*     | tVar n => ret (E.tVar n) *)
+(*     | tEvar m l => *)
+(*       l' <- monad_map (extract Σ Γ) l;; *)
+(*       ret (E.tEvar m l') *)
+(*     | tSort u => ret E.tBox *)
+(*     | tConst kn u => ret (E.tConst kn) *)
+(*     | tInd kn u => ret E.tBox *)
+(*     | tConstruct kn k u => ret (E.tConstruct kn k) *)
+(*     | tProd na b t => ret E.tBox *)
+(*     | tLambda na b t => *)
+(*       t' <- extract Σ (vass na b :: Γ) t;; *)
+(*       ret (E.tLambda na t') *)
+(*     | tLetIn na b t0 t1 => *)
+(*       b' <- extract Σ Γ b;; *)
+(*       t1' <- extract Σ (vdef na b t0 :: Γ) t1;; *)
+(*       ret (E.tLetIn na b' t1') *)
+(*     | tApp f u => *)
+(*       f' <- extract Σ Γ f;; *)
+(*       l' <- extract Σ Γ u;; *)
+(*       ret (E.tApp f' l') (* if is_dummy f' then ret dummy else *) *)
+(*     | tCase ip p c brs => *)
+(*       c' <- extract Σ Γ c;; *)
+(*       brs' <- monad_map (T:=typing_result) (fun x => x' <- extract Σ Γ (snd x);; ret (fst x, x')) brs;; *)
+(*         ret (E.tCase ip c' brs') *)
+(*     | tProj p c => *)
+(*       c' <- extract Σ Γ c;; *)
+(*       ret (E.tProj p c') *)
+(*     | tFix mfix n => *)
+(*       mfix' <- extract_mfix (@extract) Σ _ Γ _ mfix;; *)
+(*       ret (E.tFix mfix' n) *)
+(*     | tCoFix mfix n => *)
+(*       mfix' <- extract_mfix (@extract) Σ _ Γ _ mfix;; *)
+(*       ret (E.tCoFix mfix' n) *)
+(*     end. *)
 
-End Erase.
+(* End Erase. *)
 
 
-(* Definition optM {A B} (x : option A) (f : A -> B) : M (option B) := *)
-(*   match x with *)
-(*   | Some x => y <- f x ;; ret (Some y) *)
-(*   | None => ret None *)
-(*   end. *)
+(* Section Erase. *)
+(*   (* Context `{F : Fuel}. *) *)
 
-Definition extract_constant_body Σ (cb : constant_body) : E.constant_body :=
-  let ty := extract Σ [] cb.(cst_type) in
-  let body := option_map (fun b => extract Σ [] b) cb.(cst_body)  in
-  Ret {| E.cst_body := body; |}.
+(*   Definition is_box c := *)
+(*     match c with *)
+(*     | E.tBox => true *)
+(*     | _ => false *)
+(*     end. *)
 
-(* Definition lift_opt_typing {A} (a : option A) (e : type_error) : typing_result A := *)
-(*   match a with *)
-(*   | Some x => ret x *)
-(*   | None => raise e *)
-(*   end. *)
+(*   Fixpoint mkAppBox c n := *)
+(*     match n with *)
+(*     | 0 => c *)
+(*     | S n => mkAppBox (E.tApp c E.tBox) n *)
+(*     end. *)
+
+(*   Definition on_snd_map {A B C} (f : B -> C) (p : A * B) := *)
+(*     (fst p, f (snd p)). *)
+
+(*   Section EraseMfix. *)
+(*     Context (extract : forall (Γ : context) (t : term), E.term). *)
+
+(*     Definition extract_mfix Γ (defs : mfixpoint term) : (EAst.mfixpoint E.term) := *)
+(*       let Γ' := (PCUICLiftSubst.fix_context defs ++ Γ)%list in *)
+(*       map (fun d => let dbody' := extract Γ' d.(dbody) in *)
+(*                           Ret ({| E.dname := d.(dname); E.rarg := d.(rarg); *)
+(*                                   E.dbody := dbody' |})) defs. *)
+(*   End EraseMfix. *)
+  
+(*   Fixpoint extract (Σ : global_context) (Γ : context) (t : term) : E.term := *)
+(*     if is_type_or_proof Σ Γ t then E.tBox else *)
+(*     match t with *)
+(*     | tRel i => Ret (E.tRel i) *)
+(*     | tVar n => Ret (E.tVar n) *)
+(*     | tEvar m l => *)
+(*       Ret (E.tEvar m (map (extract Σ Γ) l)) *)
+(*     | tSort u => Ret E.tBox *)
+(*     | tConst kn u => Ret (E.tConst kn) *)
+(*     | tInd kn u => Ret E.tBox *)
+(*     | tConstruct kn k u => Ret (E.tConstruct kn k) *)
+(*     | tProd na b t => Ret E.tBox *)
+(*     | tLambda na b t => *)
+(*       let t' := extract Σ (vass na b :: Γ) t in *)
+(*       Ret (E.tLambda na t') *)
+(*     | tLetIn na b t0 t1 => *)
+(*       let b' := extract Σ Γ b in *)
+(*       let t1' := extract Σ (vdef na b t0 :: Γ) t1 in *)
+(*       Ret (E.tLetIn na b' t1') *)
+(*     | tApp f u => *)
+(*       let f' := extract Σ Γ f in *)
+(*       let l' := extract Σ Γ u in *)
+(*       Ret (E.tApp f' l') (* if is_dummy f' then Ret dummy else *) *)
+(*     | tCase ip p c brs => *)
+(*       let c' := extract Σ Γ c in *)
+(*       (* if is_box c' then *) *)
+(*       (*   match brs with *) *)
+(*       (*   | (n, x) :: _ => *) *)
+(*       (*     let x' := extract Σ Γ x in *) *)
+(*       (*     Ret (mkAppBox x' n) (* Singleton elimination *) *) *)
+(*       (*   | nil => *) *)
+(*       (*     Ret (E.tCase ip c' nil) (* Falsity elimination *) *) *)
+(*       (*   end *) *)
+(*       (* else *) *)
+(*         let brs' := map (B := nat * E.term) (fun x => let x' := extract Σ Γ (snd x) in Ret (fst x, x')) brs in *)
+(*         Ret (E.tCase ip c' brs') *)
+(*     | tProj p c => *)
+(*       let c' := extract Σ Γ c in *)
+(*       Ret (E.tProj p c') *)
+(*     | tFix mfix n => *)
+(*       let mfix' := extract_mfix (extract Σ) Γ mfix in *)
+(*       Ret (E.tFix mfix' n) *)
+(*     | tCoFix mfix n => *)
+(*       let mfix' := extract_mfix (extract Σ) Γ mfix in *)
+(*       Ret (E.tCoFix mfix' n) *)
+(*     end. *)
+
+(* End Erase. *)
+
+
+(* (* Definition optM {A B} (x : option A) (f : A -> B) : M (option B) := *) *)
+(* (*   match x with *) *)
+(* (*   | Some x => y <- f x ;; ret (Some y) *) *)
+(* (*   | None => ret None *) *)
+(* (*   end. *) *)
+
+(* Definition extract_constant_body Σ (cb : constant_body) : E.constant_body := *)
+(*   let ty := extract Σ [] cb.(cst_type) in *)
+(*   let body := option_map (fun b => extract Σ [] b) cb.(cst_body)  in *)
+(*   Ret {| E.cst_body := body; |}. *)
+
+(* (* Definition lift_opt_typing {A} (a : option A) (e : type_error) : typing_result A := *) *)
+(* (*   match a with *) *)
+(* (*   | Some x => ret x *) *)
+(* (*   | None => raise e *) *)
+(* (*   end. *) *)
 
 Definition opt_def {A} (a : option A) (e : A) : A :=
   match a with
@@ -184,42 +260,42 @@ Definition opt_def {A} (a : option A) (e : A) : A :=
   | None => e
   end.
 
-Definition extract_one_inductive_body (Σ : global_context) (npars : nat) (arities : context)
-           (oib : one_inductive_body) : E.one_inductive_body :=
-  let decty := opt_def (decompose_prod_n_assum [] npars oib.(ind_type)) ([], tRel 0) in
-  let '(params, arity) := decty in
-  let ctors := map (fun '(x, y, z) => let y' := Ret (extract Σ arities y) in Ret (x, y', z)) oib.(ind_ctors) in
-  let projctx := arities ,,, params ,, vass nAnon oib.(ind_type) in
-  let projs := map (fun '(x, y) => let y' := Ret (extract Σ [] y) in Ret (x, y')) oib.(ind_projs) in
-  Ret {| E.ind_name := oib.(ind_name);
-         E.ind_kelim := oib.(ind_kelim);
-         E.ind_ctors := ctors;
-         E.ind_projs := projs |}.
+(* Definition extract_one_inductive_body (Σ : global_context) (npars : nat) (arities : context) *)
+(*            (oib : one_inductive_body) : E.one_inductive_body := *)
+(*   let decty := opt_def (decompose_prod_n_assum [] npars oib.(ind_type)) ([], tRel 0) in *)
+(*   let '(params, arity) := decty in *)
+(*   let ctors := map (fun '(x, y, z) => let y' := Ret (extract Σ arities y) in Ret (x, y', z)) oib.(ind_ctors) in *)
+(*   let projctx := arities ,,, params ,, vass nAnon oib.(ind_type) in *)
+(*   let projs := map (fun '(x, y) => let y' := Ret (extract Σ [] y) in Ret (x, y')) oib.(ind_projs) in *)
+(*   Ret {| E.ind_name := oib.(ind_name); *)
+(*          E.ind_kelim := oib.(ind_kelim); *)
+(*          E.ind_ctors := ctors; *)
+(*          E.ind_projs := projs |}. *)
 
-Definition extract_mutual_inductive_body Σ
-           (mib : mutual_inductive_body) : E.mutual_inductive_body :=
-  let bds := mib.(ind_bodies) in
-  let arities := arities_context bds in
-  let bodies := map (extract_one_inductive_body Σ mib.(ind_npars) arities) bds in
-  Ret {| E.ind_npars := mib.(ind_npars);
-         E.ind_bodies := bodies; |}.
+(* Definition extract_mutual_inductive_body Σ *)
+(*            (mib : mutual_inductive_body) : E.mutual_inductive_body := *)
+(*   let bds := mib.(ind_bodies) in *)
+(*   let arities := arities_context bds in *)
+(*   let bodies := map (extract_one_inductive_body Σ mib.(ind_npars) arities) bds in *)
+(*   Ret {| E.ind_npars := mib.(ind_npars); *)
+(*          E.ind_bodies := bodies; |}. *)
 
-Fixpoint extract_global_decls univs Σ : E.global_declarations :=
-  match Σ with
-  | [] => []
-  | ConstantDecl kn cb :: Σ =>
-    let cb' := extract_constant_body (Σ, univs) cb in
-    let Σ' := extract_global_decls univs Σ in
-    E.ConstantDecl kn cb' :: Σ'
-  | InductiveDecl kn mib :: Σ =>
-    let mib' := extract_mutual_inductive_body (Σ, univs) mib in
-    let Σ' := extract_global_decls univs Σ in
-    E.InductiveDecl kn mib' :: Σ'
-  end.
+(* Fixpoint extract_global_decls univs Σ : E.global_declarations := *)
+(*   match Σ with *)
+(*   | [] => [] *)
+(*   | ConstantDecl kn cb :: Σ => *)
+(*     let cb' := extract_constant_body (Σ, univs) cb in *)
+(*     let Σ' := extract_global_decls univs Σ in *)
+(*     E.ConstantDecl kn cb' :: Σ' *)
+(*   | InductiveDecl kn mib :: Σ => *)
+(*     let mib' := extract_mutual_inductive_body (Σ, univs) mib in *)
+(*     let Σ' := extract_global_decls univs Σ in *)
+(*     E.InductiveDecl kn mib' :: Σ' *)
+(*   end. *)
 
-Definition extract_global Σ :=
-  let '(Σ, univs) := Σ in
-  extract_global_decls univs Σ.
+(* Definition extract_global Σ := *)
+(*   let '(Σ, univs) := Σ in *)
+(*   extract_global_decls univs Σ. *)
 
 Reserved Notation "Σ ;;; Γ |- s ⇝ℇ t" (at level 50, Γ, s, t at next level).
 
