extraction/theories/ErasureFunction.v
@@ -1,0 +1,343 @@
+(* Distributed under the terms of the MIT license.   *)
+
+From Coq Require Import Bool String List Program BinPos Compare_dec Omega.
+From MetaCoq.Template Require Import config utils monad_utils BasicAst AstUtils.
+From MetaCoq.PCUIC Require Import PCUICAst PCUICAstUtils PCUICInduction PCUICTyping PCUICChecker PCUICRetyping PCUICMetaTheory PCUICWcbvEval PCUICSafeChecker PCUICLiftSubst.
+From MetaCoq.Extraction Require EAst ELiftSubst ETyping EWcbvEval Extract ExtractionCorrectness.
+Require Import String.
+Local Open Scope string_scope.
+Set Asymmetric Patterns.
+Import MonadNotation.
+
+Existing Instance config.default_checker_flags.
+
+Definition is_prop_sort s :=
+  match Universe.level s with
+  | Some l => Level.is_prop l
+  | None => false
+  end.
+
+Require Import Extract.
+
+Parameter is_type_or_proof :
+  forall (Sigma : PCUICAst.global_context) (HΣ : ∥wf Sigma∥) (Gamma : context) (HΓ : ∥wf_local Sigma Gamma∥) (t : PCUICAst.term),
+    {r : typing_result bool & match r with
+                           | Checked true => Is_Type_or_Proof Sigma Gamma t 
+                           | Checked false => (Is_Type_or_Proof Sigma Gamma t -> False) × PCUICSafeLemmata.welltyped Sigma Gamma t
+                           | _ => True
+                           end}.
+
+
+Section Erase.
+
+  Definition is_box c :=
+    match c with
+    | E.tBox => true
+    | _ => false
+    end.
+
+  Fixpoint mkAppBox c n :=
+    match n with
+    | 0 => c
+    | S n => mkAppBox (E.tApp c E.tBox) n
+    end.
+
+  Definition on_snd_map {A B C} (f : B -> C) (p : A * B) :=
+    (fst p, f (snd p)).
+
+  Section EraseMfix.
+    Context (extract : forall (Σ : global_context) (wfΣ : ∥ wf Σ ∥) (Γ : context) (HΓ : ∥ wf_local Σ Γ ∥) (t : term), typing_result E.term).
+
+    Program Definition extract_mfix Σ (wfΣ : ∥wf Σ∥) Γ (HΓ : ∥wf_local Σ Γ∥) (defs : mfixpoint term) : typing_result (EAst.mfixpoint E.term) :=
+      let Γ' := (PCUICLiftSubst.fix_context defs ++ Γ)%list in
+      monad_map (fun d => H <- _ ;;
+                   dbody' <- extract Σ wfΣ Γ' H d.(dbody);;
+                          ret ({| E.dname := d.(dname); E.rarg := d.(rarg);
+                                  E.dbody := dbody' |})) defs.
+    Next Obligation.
+      clear extract.
+      
+      epose proof ((fix check_types (mfix : mfixpoint term) acc (Hacc : ∥ wf_local_rel Σ Γ acc ∥) {struct mfix}
+              : typing_result (∥ wf_local_rel Σ (Γ ,,, acc) (fix_context_i #|acc| mfix) ∥)
+              := match mfix with
+                 | [] => ret (sq wf_local_rel_nil)
+                 | def :: mfix =>
+       (* probably not tail recursive but needed so that next line terminates *)
+                   W <- infer_type infer Γ HΓ (dtype def) ;;
+                   let W' := weakening_sq acc _ _ W.π2 in
+                   Z <- check_types mfix
+                     (acc ,, vass (dname def) ((lift0 #|acc|) (dtype def)))
+                     (wf_local_rel_abs_sq Hacc (W.π1; W')) ;;
+                   ret (wf_local_rel_app_inv_sq
+                          (wf_local_rel_abs_sq (sq wf_local_rel_nil) (W.π1; W')) Z)
+                 end)
+           defs [] (sq _)).
+      destruct X. econstructor .
+      sq. eapply wf_local_local_rel.
+      eapply wf_local_rel_app_inv. eapply wf_local_rel_local. eauto.
+      change fix_context with (fix_context_i #|@nil context_decl|).
+      now rewrite app_context_nil_l.
+      sq. econstructor 2. exact t.
+      Unshelve. (* I believe those go away once infer works on squashed assumptions *)
+    Admitted.
+      
+  End EraseMfix.
+
+  Fixpoint extract (Σ : global_context) (HΣ : ∥wf Σ∥) (Γ : context) (HΓ : ∥wf_local Σ Γ∥) (t : term) {struct t} : typing_result E.term.
+  Proof.
+    destruct (is_type_or_proof Σ HΣ Γ HΓ t) eqn:E1.
+    destruct x as [b | ] eqn:E2.
+    destruct b eqn:E3.
+    - exact (ret (E.tBox)).
+    - revert y E1. refine (match t with
+             | tRel i => fun _ _ => ret (E.tRel i)
+             | tVar n => fun _ _ =>  ret (E.tVar n)
+             | tEvar m l => fun _ _ => 
+               l' <- monad_map (extract Σ HΣ Γ HΓ) l;;
+                  ret (E.tEvar m l')
+             | tSort u => fun _ _ =>  ret E.tBox
+             | tConst kn u => fun _ _ =>  ret (E.tConst kn)
+             | tInd kn u => fun _ _ =>  ret E.tBox
+             | tConstruct kn k u => fun _ _ =>  ret (E.tConstruct kn k)
+             | tProd na b t => fun _ _ =>  ret E.tBox
+             | tLambda na b t => fun _ _ => 
+               t' <- extract Σ HΣ (vass na b :: Γ) _ t;;
+                  ret (E.tLambda na t')
+             | tLetIn na b t0 t1 => fun _ _ => 
+               b' <- extract Σ HΣ Γ HΓ b;;
+                  t1' <- extract Σ HΣ (vdef na b t0 :: Γ) _ t1;;
+                  ret (E.tLetIn na b' t1')
+             | tApp f u => fun _ _ => 
+               f' <- extract Σ HΣ Γ HΓ f;;
+                  l' <- extract Σ HΣ Γ HΓ u;;
+                  ret (E.tApp f' l') (* if is_dummy f' then ret dummy else *)
+             | tCase ip p c brs => fun _ _ => 
+               c' <- extract Σ HΣ Γ HΓ c;;
+                  brs' <- monad_map (T:=typing_result) (fun x => x' <- extract Σ HΣ Γ HΓ (snd x);; ret (fst x, x')) brs;;
+                  ret (E.tCase ip c' brs')
+             | tProj p c => fun _ _ => 
+               c' <- extract Σ HΣ Γ HΓ c;;
+                  ret (E.tProj p c')
+             | tFix mfix n => fun _ _ =>  
+                 mfix' <- extract_mfix (extract) Σ HΣ Γ HΓ mfix;;
+                 ret (E.tFix mfix' n)
+             | tCoFix mfix n => fun _ _ =>  
+                 mfix' <- extract_mfix (extract) Σ HΣ Γ HΓ mfix;;
+                 ret (E.tCoFix mfix' n)
+              end).
+      
+      + destruct p as [? []]. sq. clear e.
+        Require Import MetaCoq.PCUIC.PCUICInversion. 
+        
+        eapply inversion_Lambda in t1 as (? & ? & ? & ? & ?).
+        econstructor; cbn; eauto.
+      + destruct p as [? []]. sq. clear e.
+                
+        eapply inversion_LetIn in t2 as (? & ? & ? & ? & ? & ?).
+        econstructor; cbn; eauto.
+    - exact (TypeError t0).
+  Defined.
+
+End Erase.
+
+Require Import Extract ExtractionCorrectness.
+
+Lemma erases_extract Σ Γ t T (wfΣ : ∥wf Σ∥) (wfΓ : ∥wf_local Σ Γ∥) t' :
+  Σ ;;; Γ |- t : T ->
+  extract Σ (wfΣ) Γ (wfΓ) t = Checked t' ->                
+  erases Σ Γ t t'.
+Proof.
+  Hint Constructors typing erases.
+  Hint Resolve is_type_or_proof_spec.
+  intros. sq.
+  (* pose proof (typing_wf_local X0). *)
+
+    
+  pose (wfΣ' := sq t0).
+  pose (wfΓ' := sq a).
+  change (extract Σ wfΣ' Γ wfΓ' t = Checked t') in H.
+
+  revert H.
+  generalize wfΣ' wfΓ'. clear wfΣ' wfΓ'.
+  
+  revert Σ t0 Γ a t T X t'.
+  eapply (typing_ind_env (fun Σ Γ t T =>   forall (t' : E.term) (wfΣ' : ∥ wf Σ ∥) (wfΓ' : ∥ wf_local Σ Γ ∥),
+  extract Σ wfΣ' Γ wfΓ' t = Checked t' -> Σ;;; Γ |- t ⇝ℇ t'
+         )); intros.
+
+  all: (cbn in *; repeat destruct ?;
+                                 repeat match goal with
+                                          [ H : Checked _ = Checked _ |- _ ] => inv H
+                                        | [ H : TypeError _ = Checked _ |- _ ] => inv H
+                                        | [ H : _ × PCUICSafeLemmata.welltyped _ _ _ |- _ ] => destruct H as [? []]
+                                        end; eauto); subst.
+
+  - repeat econstructor; eauto.
+  - econstructor. econstructor. clear E.
+    eapply inversion_Prod in t0 as (? & ? & ? & ? & ?).
+    split. eauto. left. econstructor.
+  - econstructor. econstructor. clear E.
+    eapply inversion_Ind in t as (? & ? & ? & ? & ? & ?).
+    split. eauto. left.
+    eapply isArity_subst_instance. eapply isArity_ind_type.
+  - econstructor.
+    eapply elim_restriction_works. intros.
+    eapply f, Is_Type_or_Proof_Proof. eauto. eauto.
+    
+    pose proof (Prelim.monad_map_All2 _ _ _ brs a1 E3).
+    
+    eapply All2_All_left in X3. 2:{ intros. destruct X4. exact e. }
+
+    eapply All2_impl.
+    eapply All2_All_mix_left. eassumption. eassumption.
+    intros. destruct H5.
+    destruct ?; inv e0. cbn. eauto.
+  - econstructor.
+
+    eapply elim_restriction_works_proj. intros.
+    eapply Is_Type_or_Proof_Proof in X2. eauto.
+
+    eauto.
+  - econstructor.
+    unfold extract_mfix in *.
+    pose proof (Prelim.monad_map_All2 _ _ _ mfix a0 E2).
+    eapply All2_impl. eapply All2_All_mix_left. eassumption. eassumption.
+
+    intros. destruct X1. cbn in *. repeat destruct ?; inv e. 
+    cbn. repeat split; eauto. 
+    eapply p. eauto. 
+  - econstructor.
+    unfold extract_mfix in *.
+    pose proof (Prelim.monad_map_All2 _ _ _ mfix a0 E2).
+    eapply All2_impl. eapply All2_All_mix_left. eassumption. eassumption.
+
+    intros. destruct X1. cbn in *. repeat destruct ?; inv e.
+    cbn. repeat split; eauto. 
+    eapply p. eauto. 
+Qed.
+
+Definition optM {M : Type -> Type} `{Monad M} {A B} (x : option A) (f : A -> M B) : M (option B) :=
+  match x with
+  | Some x => y <- f x ;; ret (Some y)
+  | None => ret None
+  end.
+
+Lemma wf_local_nil {Σ} : ∥ wf_local Σ [] ∥.
+Proof. repeat econstructor. Qed.
+
+Definition extract_constant_body Σ wfΣ (cb : constant_body) : typing_result E.constant_body :=
+  ty <- extract Σ wfΣ [] wf_local_nil cb.(cst_type) ;;
+  body <- optM cb.(cst_body) (fun b => extract Σ wfΣ [] wf_local_nil b);;
+  ret {| E.cst_body := body; |}.
+
+Definition lift_opt_typing {A} (a : option A) (e : type_error) : typing_result A :=
+  match a with
+  | Some x => ret x
+  | None => raise e
+  end.
+
+Definition extract_one_inductive_body Σ wfΣ npars arities Har
+           (oib : one_inductive_body) : typing_result E.one_inductive_body :=
+  decty <- lift_opt_typing (decompose_prod_n_assum [] npars oib.(ind_type))
+        (NotAnInductive oib.(ind_type)) ;;
+  let '(params, arity) := decty in
+  type <- extract Σ wfΣ [] wf_local_nil oib.(ind_type) ;;
+  ctors <- monad_map (fun '(x, y, z) => y' <- extract Σ wfΣ arities Har y;; ret (x, y', z)) oib.(ind_ctors);;
+  let projctx := arities ,,, params ,, vass nAnon oib.(ind_type) in
+  projs <- monad_map (fun '(x, y) => y' <- extract Σ wfΣ [] wf_local_nil y;; ret (x, y')) oib.(ind_projs);;
+  ret {| E.ind_name := oib.(ind_name);
+         E.ind_kelim := oib.(ind_kelim);
+         E.ind_ctors := ctors;
+         E.ind_projs := projs |}.
+
+Program Definition extract_mutual_inductive_body Σ wfΣ
+           (mib : mutual_inductive_body) (Hm :   ∥ wf_local Σ (arities_context (ind_bodies mib)) ∥)
+: typing_result E.mutual_inductive_body :=
+  let bds := mib.(ind_bodies) in
+  let arities := arities_context bds in
+  bodies <- monad_map (extract_one_inductive_body Σ wfΣ mib.(ind_npars) arities _) bds ;;
+  ret {| E.ind_npars := mib.(ind_npars);
+         E.ind_bodies := bodies; |}.
+
+Program Fixpoint extract_global_decls univs Σ : ∥ wf (Σ, univs) ∥ -> typing_result E.global_declarations := fun wfΣ =>
+  match Σ with
+  | [] => ret []
+  | ConstantDecl kn cb :: Σ => 
+    cb' <- extract_constant_body (Σ, univs) _ cb;;
+    Σ' <- extract_global_decls univs Σ _;;
+    ret (E.ConstantDecl kn cb' :: Σ')
+  | InductiveDecl kn mib :: Σ => 
+    mib' <- extract_mutual_inductive_body (InductiveDecl kn mib :: Σ, univs) _ mib _ ;;
+    Σ' <- extract_global_decls univs Σ _;;
+    ret (E.InductiveDecl kn mib' :: Σ')
+  end.
+Next Obligation.
+  sq. eapply PCUICWeakeningEnv.wf_extends. eauto. eexists [_]; reflexivity.
+Qed.
+Next Obligation.
+  sq. eapply PCUICWeakeningEnv.wf_extends. eauto. eexists [_]; reflexivity.
+Qed.
+Next Obligation.
+  Require Import MetaCoq.PCUIC.PCUICWeakeningEnv.
+  sq. eapply PCUICSubstitution.wf_arities_context. eauto.
+  
+  cbn. instantiate (1 := kn). unfold declared_minductive.
+  cbn. destruct (ident_eq_spec kn kn). all:try congruence.
+Qed.
+Next Obligation.
+  sq. eapply PCUICWeakeningEnv.wf_extends. eauto. eexists [_]; reflexivity.
+Qed.
+
+Program Definition extract_global Σ : ∥wf Σ∥ -> _:=
+  match Σ with (Σ, univs) => fun wfΣ  =>
+  Σ' <- extract_global_decls univs Σ wfΣ ;;
+  ret Σ' end.
+
+Lemma extract_global_correct Σ (wfΣ : ∥ wf Σ∥) Σ' :
+  extract_global Σ wfΣ = Checked Σ' ->
+  erases_global Σ Σ'.
+Proof.
+  destruct Σ as (Σ, univs).
+  induction Σ in wfΣ, Σ' |- *; cbn; intros.
+  - inv H. econstructor.
+  - repeat destruct ?; try congruence.
+    + inv H. inv E. inv E1. econstructor.
+      * unfold erases_constant_body.
+        unfold optM in E4. destruct ?; try congruence.
+        -- cbn. cbn in *.
+           destruct (         extract (Σ, univs)
+           (extract_global_decls_obligation_1 univs (ConstantDecl k c :: Σ) wfΣ k c Σ
+              eq_refl) [] wf_local_nil t
+                    ) eqn:E5;
+             rewrite E5 in E4; inv E4.
+           eapply erases_extract. 2:eauto.
+           admit.
+        -- cbn. inv E4. econstructor.
+      * eapply IHΣ. unfold extract_global. rewrite E2. reflexivity.
+    + inv H. inv E. inv E1.
+      econstructor.
+      * econstructor; cbn; eauto.
+        pose proof (Prelim.monad_map_All2 _ _ _ _ _ E3).
+        eapply All2_Forall.
+        eapply All2_impl. eassumption.
+
+        intros. cbn in H0. repeat destruct ?; try congruence.
+        inv H0. unfold erases_one_inductive_body. cbn.
+        unfold lift_opt_typing in E.
+        destruct decompose_prod_n_assum eqn:E6; inv E. cbn.
+        pose proof (Prelim.monad_map_All2 _ _ _ _ _ E4). 
+        pose proof (Prelim.monad_map_All2 _ _ _ _ _ E5). repeat split; eauto.
+        -- eapply All2_Forall.
+           eapply All2_impl. eassumption.
+           intros. destruct x0, p, y, p. cbn in *.
+           destruct ?; try congruence.
+           inv H2. split; eauto.
+           eapply erases_extract. 2:eauto. admit. admit.
+        -- eapply All2_Forall.
+           eapply All2_impl. eassumption.
+           intros. cbn in H2. destruct x0, y.
+           destruct ?; try congruence.
+           inv H2. split; eauto.
+           eapply erases_extract. 2:eauto. admit. admit.
+      * eapply IHΣ. unfold extract_global. rewrite E2. reflexivity.
+Admitted.
